src/library/tactic/simplify.h
@@ -26,6 +26,7 @@ structure simp_config :=
 (eta  : bool)
 (proj : bool)
 (iota : bool)
+(iota_eqn : bool)
 (constructor_eq : bool)
 (single_pass : bool)
 (fail_if_unchaged : bool)
@@ -43,6 +44,7 @@ struct simp_config {
     bool                      m_eta;
     bool                      m_proj;
     bool                      m_iota;
+    bool                      m_iota_eqn;
     bool                      m_constructor_eq;
     bool                      m_single_pass;
     bool                      m_fail_if_unchanged;
