library/init/meta/smt/interactive.lean
@@ -236,9 +236,9 @@ slift (tactic.interactive.induction p rec_name ids revert)
 open tactic
 
 /-- Simplify the target type of the main goal. -/
-meta def simp (no_dflt : parse only_flag) (hs : parse simp_arg_list) (attr_names : parse with_ident_list)
-              (cfg : simp_config_ext := {}) : smt_tactic unit :=
-tactic.interactive.simp no_dflt hs attr_names (loc.ns [none]) cfg
+meta def simp (use_iota_eqn : parse $ (tk "!")?) (no_dflt : parse only_flag) (hs : parse simp_arg_list)
+              (attr_names : parse with_ident_list) (cfg : simp_config_ext := {}) : smt_tactic unit :=
+tactic.interactive.simp use_iota_eqn no_dflt hs attr_names (loc.ns [none]) cfg
 
 meta def dsimp (no_dflt : parse only_flag) (es : parse simp_arg_list) (attr_names : parse with_ident_list) : smt_tactic unit :=
 tactic.interactive.dsimp no_dflt es attr_names (loc.ns [none])
