tests/lean/run/simp_iota_eqn.lean
@@ -1,0 +1,29 @@
+def f {α : Type} (a : α) : α :=
+a
+
+example (a : nat) (h : a = 3) : [1,2].map nat.succ = [2, f a] :=
+begin
+  simp!,
+  guard_target nat.succ 2 = f a,
+  simp [f, h]
+end
+
+def foo : bool → bool → bool
+| tt tt := tt
+| ff ff := tt
+| _  _  := ff
+
+example : foo tt tt = f tt :=
+begin
+  simp!,
+  guard_target tt = f tt,
+  simp [f]
+end
+
+example (b : bool) (h : b = tt) : foo b tt = f tt :=
+begin
+  fail_if_success { simp! },
+  simp! [h],
+  guard_target tt = f tt,
+  simp [f]
+end
